AP/AP/HistBlind/D.lean
@@ -37,16 +37,46 @@ theorem State.dwn_histBlind {s hist} [hs : sys.WF s] [hs' : sys.WF # s.setHist h
   · specialize @ih s' s.hist hs' d' hd' d hd s (by simp [←h₄])
       hs _ hn' H₂ H₃ _ hn h₂ h₃ (ne_symm' H')
     simp at H ih; exact H' # le_antisymm ih H
-  clear H'
-  
-  rename' d' => d₀
-  rename' hd' => hd₀
+  clear! H' d'
   
   suffices h : ∃ (d' : DStrat), d'.WF ∧ ∀ (a : AStrat), a.WF →
     (sys.simulate (Strat.f ⟨a, d'⟩) s' n).2 ≠ 0
   · specialize H₃ n h; linarith
   
-  sorry
+  generalize hd' : DStrat.mk' (λ sd => some # d.f # sd.setHistAt hist s.hist) = d'
+  have Hd' : d'.WF; rw [←hd']; infer_instance
+  
+  use d', Hd'
+  intro a Ha
+  
+  generalize ha' : AStrat.mk' (λ sa => some # a.f # sa.setHistAt s.hist hist) = a'
+  have Ha' : a'.WF; rw [←ha']; infer_instance
+  specialize h₂ a' Ha'
+  
+  have h₄' : s'.setHist s.hist = s
+  · simp [←h₄]
+  
+  contrapose! h₂
+  apply sys.simulate_congr_rel' (r := λ s₁ s₂ => s₁.setHistAt hist s.hist = s₂) h₂
+  · subst h₄; simp
+  intro k hk s₁' s₁ s₂ H₁ H₂ H₄ H₅
+  have H₄' : s₁.setHistAt s.hist hist = s₁'
+  · rw [←H₄]
+    sorry
+  have hs₁' := sys.wf_of_simulate_eq H₁
+  have hs₁ := sys.wf_of_simulate_eq H₂
+  dsimp at hs₁' hs₁
+  replace hs₁' := s₁'.aState_or_dState
+  rcases hs₁' with hs₁' | hs₁'
+  · replace hs₁ : AState s₁
+    · use hs₁; rw [←H₄]; simp
+    simp [-AState.tr_eq_some_iff] at H₅
+    use s₁'.setHistAt hist s.hist
+    simp [-AState.tr_eq_some_iff, ←ha']
+    sorry
+  · replace hs₁ : DState s₁
+    · use hs₁; rw [←H₄]; simp
+    sorry
 
 -- #check 0 #exit
 
